The poison-type based system shall work

Phi_Semantics/PhiSem_Aggregate_Tuple.thy
@@ -8,14 +8,20 @@ section \<open>Semantics\<close>
 debt_axiomatization sem_tup_T    :: \<open>TY list \<Rightarrow> TY\<close>
                 and sem_mk_tup   :: \<open>VAL list \<Rightarrow> VAL\<close>
                 and sem_dest_tup :: \<open>VAL \<Rightarrow> VAL list\<close>
-  where sem_dest_mk_tup[simp]: \<open>sem_dest_tup (sem_mk_tup vs) = vs\<close>
+                where sem_dest_mk_tup[simp]: \<open>sem_dest_tup (sem_mk_tup vs) = vs\<close>
   and   WT_tup[simp]: \<open>Well_Type (sem_tup_T ts)  = { sem_mk_tup vs |vs. list_all2 (\<lambda> t v. v \<in> Well_Type t) ts vs }\<close>
-  and   zero_tup[simp]: \<open>Zero (sem_tup_T Ts)     = map_option sem_mk_tup (those (map Zero Ts))\<close>
+  and   semty_tup_eq_poison[simp]: \<open>sem_tup_T Ts = \<p>\<o>\<i>\<s>\<o>\<n> \<longleftrightarrow> \<p>\<o>\<i>\<s>\<o>\<n> \<in> set Ts\<close>
+  and   semty_tup_uniq:
+            \<open>sem_mk_tup vs \<in> Well_Type TY \<Longrightarrow> \<exists>Ts. TY = sem_tup_T Ts\<close>
+
+  and   zero_tup[simp]: \<open>sem_tup_T Ts \<noteq> \<p>\<o>\<i>\<s>\<o>\<n> \<Longrightarrow> Zero (sem_tup_T Ts)     = map_option sem_mk_tup (those (map Zero Ts))\<close>
   and   V_tup_sep_disj_R[simp]: \<open>sem_mk_tup l1 ## vl2 \<longleftrightarrow> (\<exists>l2. vl2 = sem_mk_tup l2)\<close>
   and   V_tup_sep_disj_L[simp]: \<open>vl1 ## sem_mk_tup l2 \<longleftrightarrow> (\<exists>l1. vl1 = sem_mk_tup l1)\<close>
   and   V_tup_mult    : \<open>sem_mk_tup l1 * sem_mk_tup l2 = sem_mk_tup (l1 @ l2)\<close>
-  and   idx_step_type_tup [eval_aggregate_path] : \<open>i < length tys \<Longrightarrow> idx_step_type (AgIdx_N i) (sem_tup_T tys) = tys!i \<close>
-  and   valid_idx_step_tup[eval_aggregate_path] : \<open>valid_idx_step (sem_tup_T tys) j \<longleftrightarrow> j \<in> {AgIdx_N i | i. i < length tys}\<close>
+  and   idx_step_type_tup [eval_aggregate_path] : \<open> sem_tup_T tys \<noteq> \<p>\<o>\<i>\<s>\<o>\<n> \<and> i < length tys
+                                                \<Longrightarrow> idx_step_type (AgIdx_N i) (sem_tup_T tys) = tys!i \<close>
+  and   valid_idx_step_tup[eval_aggregate_path] : \<open> sem_tup_T tys \<noteq> \<p>\<o>\<i>\<s>\<o>\<n>
+                                                \<Longrightarrow> valid_idx_step (sem_tup_T tys) j \<longleftrightarrow> j \<in> {AgIdx_N i | i. i < length tys} \<close>
   and   idx_step_value_tup[eval_aggregate_path] : \<open>idx_step_value (AgIdx_N i) (sem_mk_tup vs) = vs!i\<close>
   and   idx_step_mod_value_tup : \<open>idx_step_mod_value (AgIdx_N i) f (sem_mk_tup vs) = sem_mk_tup (vs[i := f (vs!i)])\<close>
 
@@ -98,6 +104,21 @@ lemma semantic_tuple_constructor_N_no_use:
   unfolding Satisfiable_def
   by (simp; induct Ts; simp add: list_all2_Cons1) *)
 
+subsubsection \<open>Reduction to poison\<close>
+
+ML_file \<open>library/Ag_Tuple.ML\<close>
+
+local_setup \<open>setup_semty_tup_to_poison\<close>
+
+lemma
+  \<open>P (\<t>\<u>\<p> {\<p>\<o>\<i>\<s>\<o>\<n>}) = P \<p>\<o>\<i>\<s>\<o>\<n>\<close>
+  by simp
+
+lemma
+  \<open>P (\<t>\<u>\<p> {A, B, \<p>\<o>\<i>\<s>\<o>\<n>, C}) = P \<p>\<o>\<i>\<s>\<o>\<n>\<close>
+  by simp
+
+
 section \<open>\<phi>Type\<close>
 
 subsection \<open>Empty Tuple\<close>
@@ -106,7 +127,7 @@ subsection \<open>Empty Tuple\<close>
   where \<open>x \<Ztypecolon> Empty_Tuple \<equiv> sem_mk_tup [] \<Ztypecolon> Itself\<close>
   deriving Basic
        and Functionality
-       and \<open>Semantic_Type Empty_Tuple (sem_tup_T [])\<close>
+       and \<open>\<t>\<y>\<p>\<e>\<o>\<f> Empty_Tuple = \<t>\<u>\<p> {}\<close>
        and \<open>Semantic_Zero_Val (sem_tup_T []) Empty_Tuple ()\<close>
        and \<open>Is_Aggregate Empty_Tuple\<close>
        and Inhabited
@@ -122,15 +143,114 @@ declare [[\<phi>trace_reasoning = 0]]
   deriving Basic
        and Functional_Transformation_Functor
        and Functionality
-       and \<open>Semantic_Type T TY
-        \<Longrightarrow> Semantic_Type (Tuple_Field T) (sem_tup_T [TY])\<close>
-       and \<open>Semantic_Zero_Val TY T x
-        \<Longrightarrow> Semantic_Zero_Val (sem_tup_T [TY]) (Tuple_Field T) x \<close>
-       and \<open>Is_Aggregate (Tuple_Field T)\<close>
-       and Inhabited
 
 translations
   "_\<phi>Tuple (_\<phi>tuple_arg (\<phi>_tuple_ X))" \<rightleftharpoons> "CONST Tuple_Field X"
+
+definition Tuple_Type_Helper :: \<open>(VAL, 'x) \<phi> \<Rightarrow> TY list \<Rightarrow> bool\<close>
+  where \<open>Tuple_Type_Helper T Tys = (
+    (\<p>\<o>\<i>\<s>\<o>\<n> \<notin> set Tys \<longleftrightarrow> Inhabited T \<and> (\<exists>TY. \<forall>x v. v \<Turnstile> (x \<Ztypecolon> T) \<longrightarrow> v \<in> Well_Type TY)) \<and>
+    (\<forall>x c. c \<Turnstile> (x \<Ztypecolon> T) \<longrightarrow> (\<exists>vf. c = sem_mk_tup vf \<and> (\<p>\<o>\<i>\<s>\<o>\<n> \<notin> set Tys \<longrightarrow> list_all2 (\<lambda>t v. v \<in> Well_Type t) Tys vf)))
+)\<close>
+
+lemma semty_tup_eq_poison_rev[simp]: \<open>\<p>\<o>\<i>\<s>\<o>\<n> = sem_tup_T Ts \<longleftrightarrow> \<p>\<o>\<i>\<s>\<o>\<n> \<in> set Ts\<close>
+  by (metis semty_tup_eq_poison)
+  
+
+lemma
+  \<open> Tuple_Type_Helper U Tys
+\<Longrightarrow> \<t>\<y>\<p>\<e>\<o>\<f> U \<equiv> sem_tup_T Tys  \<close>
+  unfolding Tuple_Type_Helper_def SType_Of_def atomize_eq
+  apply auto
+  apply (smt (verit) SType_Of_not_poison WT_tup mem_Collect_eq someI_ex)
+  by (smt (verit) Eps_cong SType_Of_def SType_Of_not_poison WT_tup mem_Collect_eq)
+
+lemma
+  \<open> Tuple_Type_Helper \<lbrace> T \<rbrace> [\<t>\<y>\<p>\<e>\<o>\<f> T] \<close>
+  unfolding Tuple_Type_Helper_def Inhabited_def
+  apply auto
+  apply (metis (no_types) SType_Of_not_poison Tuple_Field.expansion typing_inhabited)
+  unfolding SType_Of_def Inhabited_def Satisfiable_def
+    apply (auto simp: split_ifs)
+  subgoal for x P TY by (rule exI[where x=\<open>\<t>\<u>\<p> {TY}\<close>], auto)
+  subgoal premises prems for x TY v
+    apply (insert prems(1)[THEN spec[where x=x], THEN spec[where x=\<open>sem_mk_tup [v]\<close>]] prems(2),
+            auto )
+    subgoal premises prems2
+      apply (insert prems2(1)[THEN semty_tup_uniq], clarsimp)
+      subgoal for TTT
+        by (rule exI[where x=\<open>hd TTT\<close>], insert prems, auto,
+            metis list.sel(1) list_all2_Cons2 sem_mk_tup_inj) . .
+  apply (smt (verit, best) SType_Of'_not_poison Satisfiable_I \<open>\<And>x v TY. \<lbrakk>\<forall>x v. (\<exists>xa. v = sem_mk_tup [xa] \<and> xa \<Turnstile> (x \<Ztypecolon> T)) \<longrightarrow> v \<in> Well_Type TY; v \<Turnstile> (x \<Ztypecolon> T)\<rbrakk> \<Longrightarrow> \<exists>TY. \<forall>x v. v \<Turnstile> (x \<Ztypecolon> T) \<longrightarrow> v \<in> Well_Type TY\<close> some_eq_imp)
+  by (smt (z3) someI2_ex)
+
+
+
+lemma
+  \<open> Tuple_Type_Helper Ts TYs
+\<Longrightarrow> Tuple_Type_Helper (\<lbrace> T \<rbrace> \<^emph> Ts) (\<t>\<y>\<p>\<e>\<o>\<f> T # TYs)  \<close>
+  unfolding Tuple_Type_Helper_def Inhabited_def Satisfiable_def
+  
+   apply (auto simp: SType_Of_def Inhabited_def Satisfiable_def)
+  apply (metis V_tup_sep_disj_L)
+  subgoal premises prems for x TY p xa TYa pa xb TYb pb proof -
+    obtain TXX where t1: \<open>TY = sem_tup_T TXX\<close>
+      using prems(1) prems(3) prems(9) semty_tup_uniq by blast
+    show ?thesis apply (rule exI[where x=\<open>sem_tup_T (TYa # TXX)\<close>]; auto)
+      by (smt (verit, best) NO_MATCH_def V_tup_mult_cons WT_tup list_all2_Cons mem_Collect_eq prems(3) prems(5) t1)
+  qed
+  apply (smt (verit) Well_Type_poison someI zero_set_def zero_set_iff)
+         apply (smt (verit, ccfv_threshold) NO_MATCH_def V_tup_mult_cons list.rel_inject(2) someI)
+
+  subgoal premises prems for x TY p TYa a b xa l2 proof -
+    obtain TH TXX where t1: \<open>TYa = sem_tup_T (TH # TXX)\<close>
+      by (smt (z3) NO_MATCH_def V_tup_mult_cons V_tup_sep_disj_L WT_tup list_all2_Cons2 mem_Collect_eq prems(1) prems(4) prems(6) prems(8) sem_mk_tup_inj semty_tup_uniq)
+    obtain xx vv where t2: \<open>vv \<Turnstile> (xx \<Ztypecolon> T) \<and> vv \<notin> Well_Type TH\<close>
+      using prems(5) by blast
+    show ?thesis
+      apply (insert \<open>\<forall>a b v.  _\<close>[THEN spec[where x=xx], THEN spec[where x=b], THEN spec[where x=\<open>sem_mk_tup (vv # l2)\<close>]],
+          auto)
+      apply (metis NO_MATCH_def V_tup_mult_cons V_tup_sep_disj_L prems(7) t2)
+      by (simp add: t1 t2)
+  qed
+
+  using V_tup_mult apply force
+  apply (smt (verit, del_insts) Well_Type_poison ex_in_conv someI_ex)
+
+  subgoal premises prems for x TY p a TYa b cb xa proof -
+    obtain cb' where t1: \<open>cb = sem_mk_tup cb'\<close>
+      using prems(1) prems(7) by presburger
+    have t2: \<open>\<exists>ca cb. sem_mk_tup (xa # cb') = ca * cb \<and> cb \<Turnstile> (b \<Ztypecolon> Ts) \<and> (\<exists>x. ca = sem_mk_tup [x] \<and> x \<Turnstile> (a \<Ztypecolon> T)) \<and> ca ## cb\<close>
+      by (metis NO_MATCH_def V_tup_mult_cons V_tup_sep_disj_L prems(7) prems(8) t1)
+    from \<open>\<forall>a b v. _\<close>[THEN spec[where x=a], THEN spec[where x=b], THEN spec[where x=\<open>sem_mk_tup (xa # cb')\<close>], THEN mp, OF t2]
+    have t3: \<open>sem_mk_tup (xa # cb') \<in> Well_Type TYa\<close> .
+    from semty_tup_uniq[OF this]
+    obtain TH TXX where t1: \<open>TYa = sem_tup_T (TH # TXX)\<close>
+      by (smt (verit, del_insts) WT_tup list_all2_Cons2 mem_Collect_eq sem_dest_mk_tup t3)
+
+    show ?thesis apply (rule exI[where x=\<open>sem_tup_T TXX\<close>]; auto)
+      by (smt (z3) NO_MATCH_def V_tup_mult_cons V_tup_sep_disj_L WT_tup list_all2_Cons mem_Collect_eq prems(1) prems(6) prems(8) sem_dest_mk_tup t1)
+  qed
+  apply (metis V_tup_mult)
+
+  subgoal premises prems for TY a b cb x proof -
+    obtain cb' where t1: \<open>cb = sem_mk_tup cb'\<close>
+      using prems(1) prems(6) by presburger
+    obtain TTT where t2: \<open>TY = sem_tup_T TTT\<close>
+      by (metis V_tup_mult V_tup_sep_disj_L prems(5) prems(6) prems(7) semty_tup_uniq t1)
+
+    obtain x1 v1 where t3: \<open>v1 \<Turnstile> (x1 \<Ztypecolon> T ) \<and> v1 \<notin> Well_Type (hd TTT)\<close>
+      using prems(4) by blast
+    obtain x2 v2 where t4: \<open>sem_mk_tup v2 \<Turnstile> (x2 \<Ztypecolon> Ts) \<and> sem_mk_tup v2 \<notin> Well_Type (sem_tup_T (tl TTT))\<close>
+      using prems(1) prems(3) by blast
+
+    show ?thesis
+      apply (insert \<open>\<forall>a b v. _\<close>[THEN spec[where x=a], THEN spec[where x=b], THEN spec[where x=\<open>sem_mk_tup (v1 # v2)\<close>]]; auto)
+      apply (smt (z3) NO_MATCH_def V_tup_mult_cons V_tup_sep_disj_R WT_tup \<open>\<And>thesis. (\<And>x2 v2. sem_mk_tup v2 \<Turnstile> (x2 \<Ztypecolon> Ts) \<and> sem_mk_tup v2 \<notin> Well_Type (sem_tup_T (tl TTT)) \<Longrightarrow> thesis) \<Longrightarrow> thesis\<close> list.sel(3) list_all2_Cons2 mem_Collect_eq prems(5) prems(7) sem_mk_tup_inj t2)
+      by (smt (verit, best) WT_tup list.sel(3) list_all2_Cons2 mem_Collect_eq sem_dest_mk_tup t2 t4)
+  qed
+  using V_tup_mult by blast 
+
 
 lemma Empty_Tuple_reduce[simp]:
   \<open>(((),a) \<Ztypecolon> Empty_Tuple \<^emph> \<lbrace> T \<rbrace>) = (a \<Ztypecolon> \<lbrace> T \<rbrace>)\<close>
