Phi_Semantics/PhiSem_Mem_C_Ag_NT.thy
@@ -342,6 +342,7 @@ lemma [\<phi>reason %\<A>sem_typ_mod_cut]:
 \<Longrightarrow> \<A>sem_typ_mod2 (\<^emph>) (semty_ntup f\<^sub>1) (semty_ntup f\<^sub>2) (semty_ntup f) \<close>
   unfolding \<A>sem_typ_mod2_def ..
 
+(*
 lemma [\<phi>reason %generalized_sematic_type_cut]:
   \<open> Generalized_Semantic_Type T TY
 \<Longrightarrow> Generalized_Semantic_Type (AgIdx_S k \<^bold>\<rightarrow> T) (semty_ntup (fmupd k TY fmempty)) \<close>
@@ -363,5 +364,6 @@ lemma [\<phi>reason %generalized_sematic_type_cut]:
   unfolding Generalized_Semantic_Type_def ..
 
 (* term \<open>\<m>\<e>\<m>[addr] \<s>\<l>\<i>\<c>\<e>[start, len] (\<m>\<e>\<m>-\<c>\<o>\<e>\<r>\<c>\<e> \<lbrace> a: A, b: B \<rbrace>)\<close> *)
+*)
 
 end
